SP1Operations/AndOperation.lean
@@ -5,62 +5,10 @@ abbrev WORD_BYTE_SIZE := 4
 @[reducible] def AndOperation (T : Type) :=
   Vector T WORD_BYTE_SIZE
 
--- namespace AndOperation
-
--- /-- `AndOperation` should result in and of all 4 limbs -/
--- def spec (cols : AndOperation (BabyBear))
---     (a b : Vector (BabyBear) WORD_BYTE_SIZE)
---     (is_real : BabyBear) : Prop :=
---   is_real ≠ 0 → ∀ i : Fin WORD_BYTE_SIZE,
---     a[i] &&& b[i] = cols[i]
-
--- /-- Constraints on `AndOperation` as extracted from the source code:
--- Sends: AirInteraction { values: [0, cols[0], a[0], b[0]], multiplicity: is_real, kind: Byte }
--- Sends: AirInteraction { values: [0, cols[1], a[1], b[1]], multiplicity: is_real, kind: Byte }
--- Sends: AirInteraction { values: [0, cols[2], a[2], b[2]], multiplicity: is_real, kind: Byte }
--- Sends: AirInteraction { values: [0, cols[3], a[3], b[3]], multiplicity: is_real, kind: Byte } -/
--- def extractedConstraints (cols : AndOperation (BabyBear))
---     (a b : Vector (BabyBear) WORD_BYTE_SIZE) (is_real : BabyBear) :
---     List (SP1Constraint) :=
---   [.byteAirInteraction (ByteOpcode.ofNat 0) cols[0] a[0] b[0] is_real,
---    .byteAirInteraction (ByteOpcode.ofNat 0) cols[1] a[1] b[1] is_real,
---    .byteAirInteraction (ByteOpcode.ofNat 0) cols[2] a[2] b[2] is_real,
---    .byteAirInteraction (ByteOpcode.ofNat 0) cols[3] a[3] b[3] is_real,]
-
-
--- /-- Cleaned up representation of the `AndOperation` constraints. -/
--- def idealizedConstraints (cols : AndOperation (BabyBear))
---     (a b : Vector (BabyBear) WORD_BYTE_SIZE) : Prop :=
---   a[0] &&& b[0] = cols[0] ∧
---   a[1] &&& b[1] = cols[1] ∧
---   a[2] &&& b[2] = cols[2] ∧
---   a[3] &&& b[3] = cols[3]
-
--- /-- The idealized constraints are logically equivalent to the extracted ones when `is_real := 1` -/
--- lemma extractedConstraints_iff_idealizedConstraints
---     (cols : AndOperation (BabyBear)) (a b : Vector (BabyBear) WORD_BYTE_SIZE) :
---     cols.extractedConstraints a b 1 ↔ cols.idealizedConstraints a b := by
---   simp [extractedConstraints, idealizedConstraints, ByteOpcode.ofNat, ByteOpcode.constrain]
---   tauto
-
--- /-- The extracted constraints on `AndOperation` imply the spec. -/
--- theorem correct (cols : AndOperation (BabyBear))
---     (a b : Vector (BabyBear) WORD_BYTE_SIZE) (is_real : BabyBear) :
---     cols.idealizedConstraints a b → cols.spec a b is_real := by
---   simp [idealizedConstraints, spec, sub_eq_zero, mul_eq_zero]
---   intros h1 h2 h3 h4 hreal i
---   match i with | 0 => ?_ | 1 => ?_ | 2 => ?_ | 3 => ?_
---   all_goals trivial
-
--- end AndOperation
-
-@[reducible] def AndOperation2 (T : Type) :=
-  Vector T WORD_BYTE_SIZE
-
-namespace AndOperation2
+namespace AndOperation
 
 /-- `AndOperation` should result in and of all 4 limbs -/
-def spec (cols : AndOperation2 (BabyBear))
+def spec (cols : AndOperation (BabyBear))
     (a b : Vector (BabyBear) WORD_BYTE_SIZE)
     (is_real : BabyBear) : Prop :=
   is_real ≠ 0 → ∀ i : Fin WORD_BYTE_SIZE,
@@ -71,17 +19,18 @@ Sends: AirInteraction { values: [0, cols[0], a[0], b[0]], multiplicity: is_real,
 Sends: AirInteraction { values: [0, cols[1], a[1], b[1]], multiplicity: is_real, kind: Byte }
 Sends: AirInteraction { values: [0, cols[2], a[2], b[2]], multiplicity: is_real, kind: Byte }
 Sends: AirInteraction { values: [0, cols[3], a[3], b[3]], multiplicity: is_real, kind: Byte } -/
-def extractedConstraints (cols : AndOperation2 (BabyBear))
-    (a b : Vector (BabyBear) WORD_BYTE_SIZE) (is_real : BabyBear) : Prop :=
-  -- TODO: what exactly should we be converting these interactions to?
-  -- Trying to say that if the interaction is real then the interaction enforces opcode semantics.
-  (is_real ≠ 0 → ByteOpcode.constrain (ByteOpcode.ofNat 0) cols[0] a[0] b[0]) ∧
-  (is_real ≠ 0 → ByteOpcode.constrain (ByteOpcode.ofNat 0) cols[1] a[1] b[1]) ∧
-  (is_real ≠ 0 → ByteOpcode.constrain (ByteOpcode.ofNat 0) cols[2] a[2] b[2]) ∧
-  (is_real ≠ 0 → ByteOpcode.constrain (ByteOpcode.ofNat 0) cols[3] a[3] b[3])
+def extractedConstraints (cols : AndOperation (BabyBear))
+    (a b : Vector (BabyBear) WORD_BYTE_SIZE) (is_real : BabyBear) :
+    List (SP1Constraint) :=
+  [
+  .sendAirInteraction_byte (.ofNat 0) cols[0] a[0] b[0] is_real,
+  .sendAirInteraction_byte (.ofNat 0) cols[1] a[1] b[1] is_real,
+  .sendAirInteraction_byte (.ofNat 0) cols[2] a[2] b[2] is_real,
+  .sendAirInteraction_byte (.ofNat 0) cols[3] a[3] b[3] is_real,
+  ]
 
 /-- Cleaned up representation of the `AndOperation` constraints. -/
-def idealizedConstraints (cols : AndOperation2 (BabyBear))
+def idealizedConstraints (cols : AndOperation (BabyBear))
     (a b : Vector (BabyBear) WORD_BYTE_SIZE) : Prop :=
   a[0] &&& b[0] = cols[0] ∧
   a[1] &&& b[1] = cols[1] ∧
@@ -90,13 +39,14 @@ def idealizedConstraints (cols : AndOperation2 (BabyBear))
 
 /-- The idealized constraints are logically equivalent to the extracted ones when `is_real := 1` -/
 lemma extractedConstraints_iff_idealizedConstraints
-    (cols : AndOperation2 (BabyBear)) (a b : Vector (BabyBear) WORD_BYTE_SIZE) :
-    cols.extractedConstraints a b 1 ↔ cols.idealizedConstraints a b := by
-  simp [extractedConstraints, idealizedConstraints, ByteOpcode.ofNat, ByteOpcode.constrain]
+    (cols : AndOperation (BabyBear)) (a b : Vector (BabyBear) WORD_BYTE_SIZE) :
+    constraintList_toProp (cols.extractedConstraints a b 1) ↔
+      cols.idealizedConstraints a b := by
+  simp [extractedConstraints, idealizedConstraints]
   tauto
 
 /-- The extracted constraints on `AndOperation` imply the spec. -/
-theorem correct (cols : AndOperation2 (BabyBear))
+theorem correct (cols : AndOperation (BabyBear))
     (a b : Vector (BabyBear) WORD_BYTE_SIZE) (is_real : BabyBear) :
     cols.idealizedConstraints a b → cols.spec a b is_real := by
   simp [idealizedConstraints, spec, sub_eq_zero, mul_eq_zero]
@@ -104,4 +54,4 @@ theorem correct (cols : AndOperation2 (BabyBear))
   match i with | 0 => ?_ | 1 => ?_ | 2 => ?_ | 3 => ?_
   all_goals trivial
 
-end AndOperation2
+end AndOperation
