SP1Operations/IsZeroOperation.lean
@@ -1,7 +1,5 @@
 import SP1Foundations
 
-import SP1Foundations
-
 structure IsZeroOperation where
   /-- The inverse of the input. -/
   inverse : U16
@@ -15,17 +13,18 @@ def spec (cols : IsZeroOperation)
   is_real = 1 → (a = 0 ↔ cols.result = 1)
 
 def constraints (cols : IsZeroOperation)
-    (a : U16) (is_real : U2) : Prop :=
-  (is_real.val * ((1 - (cols.inverse.val * a.val)) - cols.result.val)) = 0
-  ∧ (is_real.val * (cols.result.val * (cols.result.val - 1))) = 0
-  ∧ (is_real.val * (cols.result.val * (cols.result.val - 1))) = 0
-  ∧ (is_real.val * (cols.result.val * a.val)) = 0
+    (a : U16) (is_real : U2) : List (SP1Constraint) :=
+  [
+  .assertZero (is_real.val * ((1 - (cols.inverse.val * a.val)) - cols.result.val)),
+  .assertZero (is_real.val * (cols.result.val * (cols.result.val - 1))),
+  .assertZero (is_real.val * (cols.result.val * (cols.result.val - 1))),
+  .assertZero (is_real.val * (cols.result.val * a.val)),
+  ]
 
 theorem correct (cols : IsZeroOperation)
     (a : U16) (is_real : U2) :
-    cols.constraints a is_real → cols.spec a is_real := by
-  intro ⟨h1, h2, h3, h4⟩ h_is_real
-  simp [sub_eq_zero] at *
+    constraintList_toProp (cols.constraints a is_real) → cols.spec a is_real := by
+  simp [constraints, spec, sub_eq_zero]
   aesop
 
 end IsZeroOperation
