SP1Foundations.lean
@@ -1,4 +1,5 @@
 import SP1Foundations.ByteOpcode
+import SP1Foundations.Constraint
 import SP1Foundations.Field
 import SP1Foundations.Unsigned
 import SP1Foundations.Word
