SP1Foundations/Constraint.lean
@@ -1,0 +1,39 @@
+import SP1Foundations.Field
+import SP1Foundations.ByteOpcode
+
+inductive SP1Constraint where
+  /-- Assertion that a particular value is real. -/
+  | assertZero (x : BabyBear)
+  /-- Sending air interactions with `kind == byte` -/
+  | sendAirInteraction_byte (op : ByteOpcode)
+      (x y z : BabyBear) (mult : ℕ)
+  -- TODO: other air interactions
+
+namespace SP1Constraint
+
+def toProp : SP1Constraint → Prop
+  | .assertZero x => (x = 0)
+  | .sendAirInteraction_byte op x y z mult =>
+      -- Is this saying enough?
+      (mult ≠ 0 → ByteOpcode.constrain op x y z)
+
+@[simp] lemma toProp_assertZero (x : BabyBear) :
+    (assertZero x).toProp ↔ x = 0 := Iff.rfl
+
+@[simp] lemma toProp_sendAirInteration_byte (op : ByteOpcode)
+    (x y z : BabyBear) (mult : ℕ) :
+    (sendAirInteraction_byte op x y z mult).toProp ↔
+      (mult ≠ 0 → ByteOpcode.constrain op x y z) := Iff.rfl
+
+end SP1Constraint
+
+@[reducible] def constraintList_toProp (cs : List SP1Constraint) : Prop :=
+  ∀ constraint ∈ cs, constraint.toProp
+
+@[simp] lemma constraintList_toProp_nil :
+    constraintList_toProp [] = True := by
+  simp [constraintList_toProp]
+
+@[simp] lemma constraintList_toProp_cons (c : SP1Constraint) (cs : List SP1Constraint) :
+    constraintList_toProp (c :: cs) = (c.toProp ∧ constraintList_toProp cs) := by
+  simp [constraintList_toProp]
